HoareLogic/ImperativeLanguage.v
@@ -5,58 +5,32 @@ Class ImperativeProgrammingLanguage: Type := {
   cmd: Type
 }.
 
-Class BigStepSemantics (Imp: ImperativeProgrammingLanguage) (MD: Model): Type := {
-  state := model;
-  exceptional_state: Type;
-  access: state + exceptional_state -> cmd -> state + exceptional_state -> Prop
+Inductive MetaState (state: Type): Type :=
+  | Error: MetaState state
+  | NonTerminating: MetaState state
+  | Terminating: state -> MetaState state.
+
+Arguments Error {_}.
+Arguments NonTerminating {_}.
+Arguments Terminating {_} _.
+
+Class BigStepSemantics (Imp: ImperativeProgrammingLanguage) (state: Type): Type := {
+  access: state -> cmd -> MetaState state -> Prop
 }.
 
-(*
+Definition safe {Imp: ImperativeProgrammingLanguage} {state: Type} {BSS: BigStepSemantics Imp state} (s: state) (c: cmd): Prop :=
+  ~ access s c Error.
 
-Class FrameBigStepSemantics (Imp: ImperativeProgrammingLanguage) (MD: Model) {kMD: KripkeModel MD} {SA: forall M: Kmodel, SeparationAlgebra MD M} (BSS: BigStepSemantics Imp MD): Type := {
-  frame_property: forall 
-}.
-*)
-(*
-Class NormalImperativeProgrammingLanguage (Imp: ImperativeProgrammingLanguage): Type := {
-  Ssequence: cmd -> cmd -> cmd;
-  Sskip: cmd;
-  neq_Sskip_Ssequence: forall c1 c2, Sskip <> Ssequence c1 c2
+Definition term_norm {Imp: ImperativeProgrammingLanguage} {state: Type} {BSS: BigStepSemantics Imp state} (s: state) (c: cmd): Prop :=
+  ~ access s c Error /\ ~ access s c NonTerminating.
+
+Class NormalBigStepSemantics (Imp: ImperativeProgrammingLanguage) (state: Type) (BSS: BigStepSemantics Imp state): Type := {
+  access_defined: forall s c, exists ms, access s c ms
 }.
 
-Class SmallStepSemantics (Imp: ImperativeProgrammingLanguage) (MD: Model): Type := {
-  state := model;
-  exceptional_state: Type;
-  step: cmd * state -> cmd * state + exceptional_state -> Prop
+Class SABigStepSemantics (Imp: ImperativeProgrammingLanguage) (state: Type) {SA: SeparationAlgebra state} (BSS: BigStepSemantics Imp state): Type := {
+  safety_preserve: forall m mf m' c, join m mf m' -> safe m c -> safe m' c;
+  terminate_preserve: forall m mf m' c, join m mf m' -> term_norm m c -> term_norm m' c;
+  frame_property: forall m mf m' c n', join m mf m' -> safe m c -> access m' c (Terminating n') -> exists n, join n mf n' /\ access m c (Terminating n)
 }.
 
-Definition fmap_sum_left {A1 A2 B: Type} (f: A1 -> A2) (x: A1 + B): A2 + B :=
-  match x with
-  | inl a => inl (f a)
-  | inr b => inr b
-  end.
-
-Definition fmap_Sseq {Imp: ImperativeProgrammingLanguage} {nImp: NormalImperativeProgrammingLanguage Imp} {MD: Model} {sss: SmallStepSemantics Imp MD} (mcs: cmd * state + exceptional_state) (c0: cmd) :=
-  fmap_sum_left (fun cs: cmd * state => let (c, s) := cs in (Ssequence c c0, s)) mcs.
-
-Definition fmap_pair_cmd {Imp: ImperativeProgrammingLanguage} {nImp: NormalImperativeProgrammingLanguage Imp} {MD: Model} {sss: SmallStepSemantics Imp MD} (ms: state + exceptional_state) (c: cmd) :=
-  fmap_sum_left (pair c) ms.
-
-Class NormalSmallStepSemantics (Imp: ImperativeProgrammingLanguage) {nImp: NormalImperativeProgrammingLanguage Imp} (MD: Model) (sss: SmallStepSemantics Imp MD): Type := {
-  step_Ssequence1: forall c1 c2 s1 mcs2,
-    c2 <> Sskip ->
-    ((exists mcs1, step (c1, s1) mcs1 /\ mcs2 = fmap_Sseq mcs1 c2) <->
-     step (Ssequence c1 c2, s1) mcs2);
-  step_Ssequence2: forall c s mcs,
-    step (c, s) mcs <->
-    step (Ssequence Sskip c, s) mcs;
-  step_progress: forall c s, c = Sskip <-> exists mcs, step (c, s) mcs
-}.
-
-Inductive iter_step {Imp: ImperativeProgrammingLanguage} {nImp: NormalImperativeProgrammingLanguage Imp} {MD: Model} {sss: SmallStepSemantics Imp MD}: cmd * state + exceptional_state -> cmd * state + exceptional_state -> Prop :=
-| iter_step_refl: forall mcs, iter_step mcs mcs
-| iter_step_step: forall cs mcs1 mcs2, step cs mcs1 -> iter_step mcs1 mcs2 -> iter_step (inl cs) mcs2.
-
-Definition access {Imp: ImperativeProgrammingLanguage} {nImp: NormalImperativeProgrammingLanguage Imp} {MD: Model} {sss: SmallStepSemantics Imp MD} (ms_init: state + exceptional_state) (c: cmd) (ms_end: state + exceptional_state): Prop :=
-  iter_step (fmap_pair_cmd ms_init c) (fmap_pair_cmd ms_end Sskip).
-*)
